backend/Conventions.v
@@ -148,7 +148,8 @@ Program Definition cc_locset: callconv li_c li_locset :=
       fun '(cq id1 sg args m1) '(lq id2 rs m2) =>
         id1 = id2 /\
         args = map (fun p => Locmap.getpair p rs) (loc_arguments sg) /\
-        m1 = m2;
+        m1 = m2 /\
+        (forall l, Val.has_type (rs l) (Loc.type l));
     match_reply_def w :=
       fun '(cq _ sg _ _) '(lq _ rs _) '(res, m1) '(rs', m2) =>
         agree_callee_save rs rs' /\
@@ -165,6 +166,7 @@ Notation ls_mem w := (cq_mem (world_q1 w)).
 Lemma match_query_cc_locset (P: _->_->_->_->_->_->_-> Prop):
   (forall id sg args rs m,
    args = map (fun p => Locmap.getpair p rs) (loc_arguments sg) ->
+   (forall l, Val.has_type (rs l) (Loc.type l)) ->
    P id sg args rs m (cq id sg args m) (lq id rs m)) ->
   (forall w q1 q2, match_query cc_locset w q1 q2 ->
    P (ls_id w) (ls_sg w) (ls_args w) (ls_rs w) (ls_mem w) q1 q2).
@@ -172,7 +174,7 @@ Proof.
   intros H w q1 q2 Hq.
   destruct Hq as [w q1 q2 Hq].
   destruct q1 as [id1 sg args m1], q2 as [id2 rs m2].
-  destruct Hq as (Hid & Hargs & Hm).
+  destruct Hq as (Hid & Hargs & Hm & Hwt).
   simpl in *; subst.
   eauto.
 Qed.
